SQIR/NDSem.v
@@ -114,12 +114,15 @@ Proof.
         Msimpl; simpl;
         apply sqrt_0
       ).
+      try apply norm_zero_iff_zero. try apply WF_Zero. try easy.
     + contradict H0. 
       rewrite <- Mmult_assoc.
       rewrite proj_twice_neq by easy.
       unfold norm. 
       Msimpl; simpl.
       try apply sqrt_0.
+      try apply norm_zero_iff_zero. try apply WF_Zero.
+      try easy.
     + rewrite <- Mmult_assoc in H0, H1.
       rewrite proj_twice_eq in H0, H1.
       apply nd_meas_f; assumption.
